{
 "cells": [
  {
   "cell_type": "code",
   "execution_count": null,
   "id": "34452a2e",
   "metadata": {},
   "outputs": [],
   "source": [
    "import pymupdf\n",
    "from PIL import Image\n",
    "from LLM_wrap import LLM, img_to_b64\n",
    "from utilities import read_file"
   ]
  },
  {
   "cell_type": "code",
   "execution_count": 8,
   "id": "8cb47f1d",
   "metadata": {},
   "outputs": [],
   "source": [
    "model = \"gpt-4.1-mini\"\n",
    "gpt = LLM(model)"
   ]
  },
  {
   "cell_type": "code",
   "execution_count": 30,
   "id": "c2d06ad5",
   "metadata": {},
   "outputs": [],
   "source": [
    "direc = \"R4\"\n",
    "doc = pymupdf.open(\"./pdfs/exos R4/Série 1 - Exercice.pdf\")\n",
    "n = 0"
   ]
  },
  {
   "cell_type": "code",
   "execution_count": 31,
   "id": "14e7cf86",
   "metadata": {},
   "outputs": [
    {
     "name": "stdout",
     "output_type": "stream",
     "text": [
      "response:\n",
      "```latex\n",
      "\\documentclass{article}\n",
      "\\usepackage[utf8]{inputenc}\n",
      "\\usepackage{amsmath}\n",
      "\n",
      "\\begin{document}\n",
      "\n",
      "\\textbf{Analyse 1 - Série 1}\n",
      "\n",
      "\\textbf{Exercice 1}\n",
      "\n",
      "a) \\quad $(x+13)(x-11) \\implies x^2 - 11x + 13x - 143$ \\\\\n",
      "\\quad $\\implies x^2 + 2x - 143$ \\checkmark\n",
      "\n",
      "b) \\quad $(2x-5)(6x+3) \\implies 12x^2 + 6x - 30x - 15$ \\\\\n",
      "\\quad $\\implies 12x^2 - 24x - 15$ \\checkmark\n",
      "\n",
      "c) \\quad $(-3bc - 4b)(5bc - 5c) \\implies -15b^2c^2 + 15bc^2 - 20bc + 20bc$ \\checkmark\n",
      "\n",
      "d) \\quad $(-s^2 + 3s - 1)(2s + 9) \\implies -2s^3 - 9s^2 + 6s^2 + 27s - 2s - 9$ \\\\\n",
      "\\quad $\\implies -2s^3 - 3s^2 + 25s - 9$ \\checkmark\n",
      "\n",
      "e) \\quad $(a+b)(a-b) \\implies a^2 - ab + ba - b^2$ \\\\\n",
      "\\quad $\\implies a^2 - b^2$ \\checkmark\n",
      "\n",
      "f) \\quad $(a-b)(a^2 + ab + b^2) \\implies a^3 + a^2b + ab^2 - b a^2 - b^2 a - b^3$ \\\\\n",
      "\\quad $\\implies a^3 - b^3$ \\checkmark\n",
      "\n",
      "g) \\quad $(x-1)(1 + x + x^2 + x^3) \\implies x + x^2 + x^3 + x^4 - x - x^2 - x^3$ \\\\\n",
      "\\quad $\\implies x^4 - 1$ \\checkmark\n",
      "\n",
      "h) \\quad $(x^3 - x^2 + x - 1)(x^3 + x^2 + x + 1)$ \\\\\n",
      "\\quad $\\implies x^6 + x^5 + x^4 + x^3 - x^5 - x^4 - x^3 - x^2 + x^4 + x^3 + x^2 + x - x^3 - x^2 - x - 1$ \\\\\n",
      "\\quad $\\implies x^6 + x - 1$ \\checkmark\n",
      "\n",
      "\\end{document}\n",
      "```\n",
      "yay\n",
      "response:\n",
      "```latex\n",
      "\\documentclass{article}\n",
      "\\usepackage[utf8]{inputenc}\n",
      "\\usepackage{amsmath}\n",
      "\n",
      "\\begin{document}\n",
      "\n",
      "Exercice 2\n",
      "\n",
      "a) \\quad $(p - 7)^2 \\Rightarrow (p - 7)(p - 7) \\Rightarrow p^2 - 7p - 7p + 49 \\Rightarrow p^2 - 14p + 49$ \\quad $\\checkmark$\n",
      "\n",
      "b) \\quad $(2x + 3)^2 = (2x + 3)(2x + 3) \\Rightarrow 4x^2 + 6x + 6x + 9 \\Rightarrow 4x^2 + 12x + 9$ \\quad $\\checkmark$\n",
      "\n",
      "c) \\quad $(25p + 9q)^2 = (25p + 9q)(25p + 9q) = 625p^2 + 225pq + 225pq + 81q^2 = 625p^2 + 450pq + 81q^2$ \\quad $\\checkmark$\n",
      "\n",
      "d) \\quad $(8u^2 - 9v^2)^2 = (8u^2 - 9v^2)(8u^2 - 9v^2) = 64u^4 - 72u^2v^2 - 72u^2v^2 + 81v^4 = 64u^4 - 144u^2v^2 + 81v^4$ \\quad $\\checkmark$\n",
      "\n",
      "e) \\quad $(9p^8 + 8p)(9p^8 - 8p) = 81p^{16} - 64p^2$ \\quad $\\checkmark$\n",
      "\n",
      "f) \\quad $(2x^2 + 1)(1 - 2x^2) = 2x^2 - 4x^4 + 1 - 2x^2 = -4x^4 + 1$ \\quad $\\checkmark$\n",
      "\n",
      "g) \\quad $(2x - 1)(4x + 14) = 8x^2 + 28x - 4x - 14 = 8x^2 + 24x - 14$ \\quad $\\checkmark$\n",
      "\n",
      "h) \\quad $(2a + 3b + x)(2a + 3b + x) = 4a^2 + 6ab + 2ax + 6ab + 9b^2 + 3bx + 2ax + 3bx + x^2 = 4a^2 + 12ab + 9b^2 + 4ax + 6bx + x^2$ \\quad $\\checkmark$\n",
      "\n",
      "i) \\quad $(8u^4 - v^4)(8u^4 - v^4) = 64u^8 - 8u^4v^4 - 8u^4v^4 + v^8 = 64u^8 - 16u^4v^4 + v^8$ \\quad $\\checkmark$\n",
      "\n",
      "j) \\quad $(a + b + c)(a + b + c) = a^2 + ab + ac + ab + b^2 + bc + ac + bc + c^2$ \\\\\n",
      "\\quad $(a - b - c)(a - b - c) = a^2 - ab - ac - ab + b^2 + bc - ac + bc + c^2$ \\\\\n",
      "\\quad $\\Rightarrow 4ab + 4ac$ \\quad $\\checkmark$\n",
      "\n",
      "\\end{document}\n",
      "```\n",
      "yay\n",
      "response:\n",
      "```latex\n",
      "\\documentclass{article}\n",
      "\\usepackage[utf8]{inputenc}\n",
      "\\usepackage{amsmath}\n",
      "\n",
      "\\begin{document}\n",
      "\n",
      "Exercice 3\n",
      "\n",
      "a) \\quad 2a(a-b) - c(a-b) \\Rightarrow (a-b)(2a-c)\n",
      "\n",
      "b) \\quad 20p^2q^3 - 10p^3q^2 \\Rightarrow 10p^2q^2(2q - p)\n",
      "\n",
      "c) \\quad 14ab + 49b^2 + a^2 \\Rightarrow (a + 7b)^2\n",
      "\n",
      "d) \\quad 4c^2 - 9d^2 \\Rightarrow (2c - 3d)(2c + 3d) \\quad \\text{dédution}\n",
      "\n",
      "e) \\quad a^2 - (c^2 + 2ab) + b^2 \\Rightarrow a^2 - c^2 - 2ab + b^2 = (a - b + c)(a - b - c) \\quad \\text{Testez} \\quad *\n",
      "\n",
      "f) \\quad 7(4a - 3) - 4a + 3 \\Rightarrow 28a - 21 - 4a + 3 \\Rightarrow 24a - 18 \\Rightarrow 6(4a - 3) \\quad *\n",
      "\n",
      "g) \\quad 2(p^3 - q^3) - p^3 + q^3 = 2p^3 - 2q^3 - p^3 + q^3 = p^3 - q^3 = (p - q)(p^2 + pq + q^2)\n",
      "\n",
      "h) \\quad a^2 - b^2 \\times y^2 + 2(ax - by) \\Rightarrow (a - b \\times x - y)(a + b + x + y) \\quad *\n",
      "\n",
      "i) \\quad a^2 + 8a + 15 = (a + 5)(a + 3)\n",
      "\n",
      "j) \\quad b^2 - 29b + 208 \\Rightarrow (b - 13)(b - 16)\n",
      "\n",
      "k) \\quad 8a^3 - 27b^3 = (a - b)(a^2 + ab + b^2) \\quad * \\triangle\n",
      "\n",
      "\\quad \\Rightarrow (2a - 3b)(4a^2 + 6ab + 9b^2)\n",
      "\n",
      "\\quad 8a^3 + 12a^2b + 18ab^2 - 12a^2b - 18b^3 = 27b^3\n",
      "\n",
      "l) \\quad 8a^3 + 12a^2b + 6ab^2 + b^3 \\Rightarrow (2a + b)^3 \\quad * \\quad \\text{Apprendre pour 3\\textsuperscript{e} degré}\n",
      "\n",
      "\\end{document}\n",
      "```\n",
      "yay\n",
      "response:\n",
      "```latex\n",
      "\\documentclass{article}\n",
      "\\usepackage[utf8]{inputenc}\n",
      "\\usepackage{amsmath}\n",
      "\n",
      "\\begin{document}\n",
      "\n",
      "Exercice 4\n",
      "\n",
      "a) \\quad \n",
      "\\[\n",
      "a^2 x - 2 b^2 y + 2 a^2 y - b^3 x \\Rightarrow \\boxed{\\frac{(a^2 - b^2)(x + 2 y)}{}}\n",
      "\\]\n",
      "\n",
      "b) \\quad \n",
      "\\[\n",
      "a^2 - b^2 - 24 a x + 6 b y + 144 x^2 - 9 y^2 \\Rightarrow \\boxed{(a - 12 x - b + 3 y)(a - 12 x + b - 3 y)}\n",
      "\\]\n",
      "\n",
      "c) \\quad \n",
      "\\[\n",
      "(x^2 + 2)^2 + 4 x (x^2 + 2) + 4 x^2\n",
      "\\]\n",
      "\\[\n",
      "\\Rightarrow (x^2 + 2)(x^2) \\times x^2 + 4 \\times 9\n",
      "\\]\n",
      "\\[\n",
      "\\Rightarrow x^4 + 4 x^2 + 4 x^2 + 8 x + 4 x^2\n",
      "\\]\n",
      "\\[\n",
      "\\Rightarrow x^4 + 8 x^2 + 8 x + 4 x^2\n",
      "\\]\n",
      "\\[\n",
      "\\Rightarrow (x^2 + 2 x + 2)(x^2 + 2 x + 2)\n",
      "\\]\n",
      "\n",
      "d) \\quad \n",
      "\\[\n",
      "x^6 - 12 x^4 + 48 x^2 - 64\n",
      "\\]\n",
      "\\[\n",
      "\\Rightarrow (x - 2)^3 (x + 2)^3\n",
      "\\]\n",
      "\n",
      "\\end{document}\n",
      "```\n",
      "yay\n",
      "response:\n",
      "```latex\n",
      "\\documentclass{article}\n",
      "\\usepackage{amsmath}\n",
      "\\usepackage{amssymb}\n",
      "\\begin{document}\n",
      "\n",
      "Exercice 5\n",
      "\n",
      "a) \\quad \n",
      "\\frac{2q^2 - 4q}{3q - 1} + \\frac{3 - 9 + q^2}{3q - 1} \n",
      "\\quad \\longrightarrow \\quad \n",
      "\\frac{2q^2 - 4q + 3 - 9 + q^2}{3q - 1} \n",
      "\\quad \\text{\\small (L'addition avec tout ce polynôme donc changement de signe)}\n",
      "\n",
      "b) \\quad \n",
      "\\frac{3q - 4}{a + b} - \\frac{3q - 4}{b - a} \n",
      "\\quad \\longrightarrow \\quad \n",
      "\\frac{b - a}{(a + b)(b - a)} - \\frac{a + b}{(a + b)(b - a)} \n",
      "\\quad = \\quad \n",
      "\\frac{b - a - (a + b)}{(a + b)(b - a)} \n",
      "\\quad = \\quad \n",
      "\\frac{b - a - a - b}{(a + b)(b - a)} \n",
      "\\quad = \\quad \n",
      "\\frac{-2a}{(a + b)(b - a)}\n",
      "\n",
      "\\quad \\text{ou} \\quad \n",
      "\\frac{b - a + a + b}{(a + b)(b - a)} = \\frac{2b}{b^2 - a^2}\n",
      "\n",
      "c) \\quad \n",
      "\\frac{1}{x^6} + \\frac{1}{x^7} - \\frac{1}{x} \n",
      "\\quad \\longrightarrow \\quad \n",
      "\\frac{1}{x^6} + \\frac{1}{x^7} - \\frac{1}{x^6} \n",
      "\\quad = \\quad \n",
      "\\frac{x}{x^7} + \\frac{1}{x^7} - \\frac{x^6}{x^6} \n",
      "\\quad = \\quad \n",
      "\\frac{x + 1 - x^6}{x^6}\n",
      "\n",
      "\\quad \\text{mettre tous au même dénominateur} \\quad \\Delta\n",
      "\n",
      "d) \\quad \n",
      "\\frac{u + v}{n} - \\frac{v}{n} + \\frac{v}{n} \n",
      "\\quad \\longrightarrow \\quad \n",
      "\\frac{(u + v)(v - 1)}{uv - v^2} - \\frac{v(u - v)}{uv - v^2} + \\frac{uv - v^2}{uv - v^2} \n",
      "\\quad = \\quad \n",
      "\\frac{u v + v^2 - u v - v^2 + u v - v^2}{uv - v^2} \n",
      "\\quad = \\quad \n",
      "\\frac{u v - v^2}{uv - v^2} \n",
      "\\quad = \\quad 1\n",
      "\n",
      "e) \\quad \n",
      "\\frac{m}{n} - \\frac{n}{m} \n",
      "\\quad \\longrightarrow \\quad \n",
      "\\frac{m(m - n)}{m n} - \\frac{n(m - n)}{m n} \n",
      "\\quad = \\quad \n",
      "\\frac{m^2 - m n - n m + n^2}{m n} \n",
      "\\quad = \\quad \n",
      "\\frac{m^2 - 2 m n + n^2}{m n} \n",
      "\\quad = \\quad \n",
      "\\frac{(m - n)^2}{m n}\n",
      "\n",
      "f) \\quad \n",
      "\\frac{x - 1}{x^2 - 1} - \\frac{x + 1}{x^2 - 1} \n",
      "\\quad \\longrightarrow \\quad \n",
      "\\frac{(x - 1)(x + 1)}{(x - 1)(x + 1)} - \\frac{(x + 1)(x - 1)}{(x - 1)(x + 1)} \n",
      "\\quad = \\quad 0\n",
      "\n",
      "g) \\quad \n",
      "\\frac{4x - 12}{x^2 - 9} - \\frac{2x - 6}{x^2 - 9} \n",
      "\\quad \\longrightarrow \\quad \n",
      "\\frac{4(x - 3)}{(x - 3)(x + 3)} - \\frac{2(x - 3)}{(x - 3)(x + 3)} \n",
      "\\quad = \\quad \n",
      "\\frac{4}{x + 3} - \\frac{2}{x + 3} \n",
      "\\quad = \\quad \n",
      "\\frac{2}{x + 3}\n",
      "\n",
      "\\end{document}\n",
      "```\n",
      "yay\n",
      "response:\n",
      "```latex\n",
      "\\documentclass{article}\n",
      "\\usepackage[utf8]{inputenc}\n",
      "\\usepackage{amsmath}\n",
      "\n",
      "\\begin{document}\n",
      "\n",
      "Exercice 6\n",
      "\n",
      "a) \\quad \\frac{5a}{6b} - \\frac{3b}{10a} = \\frac{15ab}{60ab} - \\frac{18ab}{60ab} = \\frac{-3ab}{60ab} = -\\frac{1}{20}\n",
      "\n",
      "b) \\quad \\frac{72uv^2}{8u^2v} - \\frac{42t^2s}{14ts^2} = \\frac{9v}{u} - 3t = 9v - 3t\n",
      "\n",
      "c) \\quad \\frac{2u+v}{u-v} - \\frac{u-v}{4u+2v} = \\frac{(2u+v)(4u+2v)}{(u-v)(4u+2v)} - \\frac{(u-v)^2}{(u-v)(4u+2v)} = \\frac{(2u+v)(4u+2v) - (u-v)^2}{(u-v)(4u+2v)}\n",
      "\n",
      "d) \\quad \\frac{(x^2 - y^2)}{3x y - 3x^2} = \\frac{6x}{6x((x+y)(x-y))} - 2(x+y)\n",
      "\n",
      "e) \\quad \\frac{x^2 - 4x - 5}{x^2 - 9} = \\frac{(x+1)(x-5)}{(x+3)(x-3)} = 2.5\n",
      "\n",
      "f) \\quad 2x^2 + 2x - 143 = (2x+13)(2x-11) \\quad \\text{et} \\quad 2x^2 + 202 = (2x+13)(2x+15) \\quad \\Rightarrow \\quad \\frac{(2x+13)(2x-11)}{(2x+13)(2x+15)} = \\frac{2x-11}{2x+15}\n",
      "\n",
      "g) \\quad \\left(\\frac{2}{x-1} + 1\\right) \\left(\\frac{x}{x^2-1} - \\frac{2x}{x+1}\\right) = \\left(\\frac{2}{x-1} + \\frac{x-1}{x-1}\\right) \\left(\\frac{x}{(x-1)(x+1)} - \\frac{2x}{x+1}\\right)\n",
      "\n",
      "\\quad = \\left(\\frac{x+1}{x-1}\\right) \\left(\\frac{x}{(x-1)(x+1)} - \\frac{2x(x-1)}{(x+1)(x-1)}\\right)\n",
      "\n",
      "\\quad = \\left(\\frac{x+1}{x-1}\\right) \\left(\\frac{x - 2x(x-1)^2}{(x-1)(x+1)}\\right)\n",
      "\n",
      "\\quad = \\frac{(x+1)(x - 2x(x-1)^2)}{(x-1)(x-1)(x+1)} = \\frac{1}{(x^2 + 1)}\n",
      "\n",
      "\\end{document}\n",
      "```\n",
      "yay\n",
      "response:\n",
      "```latex\n",
      "\\documentclass{article}\n",
      "\\usepackage[utf8]{inputenc}\n",
      "\\usepackage{amsmath}\n",
      "\n",
      "\\begin{document}\n",
      "\n",
      "Exercice 7\n",
      "\n",
      "a) \\quad\n",
      "\\[\n",
      "\\frac{y^{-3}}{10a} = \\frac{y^3}{10a} \\quad \\frac{15b}{10a} = \\frac{15b}{10a} = \\frac{3b}{2a} \\quad \\frac{y^{-3}}{x^5}\n",
      "\\]\n",
      "\n",
      "b) \\quad\n",
      "\\[\n",
      "\\frac{x}{x} - \\frac{1}{x} \\quad \\left| \\quad \\frac{x^2 - 1}{x^2 + 1}\n",
      "\\right.\n",
      "\\]\n",
      "\n",
      "c) \\quad\n",
      "\\[\n",
      "\\frac{a+1}{a-1} \\quad \\left| \\quad (a-1) \\quad \\Rightarrow \\quad \\frac{(a+1) - a + 1}{(a+1) + a - 1} \\quad \\frac{2}{2a} \\quad \\frac{1}{a}\n",
      "\\]\n",
      "\n",
      "d) \\quad\n",
      "\\[\n",
      "\\frac{3a^2 - 2b}{6a + 12} \\quad \\frac{3(2a - 9)}{6(a+2)} \\quad \\frac{3(a\\sqrt{3}a - 3)}{6 \\times a \\sqrt{3}} \\quad \\frac{(a\\sqrt{2})(a+2)}{6(a-3)} \\quad \\frac{3(a \\times \\sqrt{3})(a+2)}{2(a-3)}\n",
      "\\]\n",
      "\n",
      "e) \\quad\n",
      "\\[\n",
      "\\frac{a^2}{a^2} - \\frac{b^2}{b^2} = \\left(\\frac{a}{b}\\right)^2 \\quad \\frac{a}{b} - \\frac{b}{a} = \\frac{a}{b} - \\frac{b}{a}\n",
      "\\]\n",
      "\n",
      "\\end{document}\n",
      "```\n",
      "yay\n",
      "response:\n",
      "```latex\n",
      "\\documentclass{article}\n",
      "\\usepackage[utf8]{inputenc}\n",
      "\\usepackage{amsmath}\n",
      "\n",
      "\\begin{document}\n",
      "\n",
      "Exercice 8\n",
      "\n",
      "a) \\[\n",
      "\\frac{ax^2+b}{2x-1} \\quad \\frac{2(ax+ax^2)}{1-4x^2} \\quad \\frac{ax^2-b}{2x-1} = \\frac{(ax^2+b)(2bx)+(2bx+2ax^2)-(ax^2-b)(2x-1)}{(2x-1)(2x+1)}\n",
      "\\]\n",
      "\n",
      "\\[\n",
      "= \\frac{2ax^2 + 9x^2 + 2bx + b - 2bx - 2ax^2 - 2bx + 2bx}{4x^2 - 1}\n",
      "\\]\n",
      "\n",
      "\\[\n",
      "= \\frac{2bx}{4x^2 - 1}\n",
      "\\]\n",
      "\n",
      "\\[\n",
      "\\boxed{\\frac{2bx}{4x^2 - 1}}\n",
      "\\]\n",
      "\n",
      "b) \\[\n",
      "\\frac{1}{(a-b)(a-c)} - \\frac{1}{(b-c)(a-c)} = \\frac{1}{(a-b)(b-c)} - \\frac{1}{(a-c)(b-c)}\n",
      "\\]\n",
      "\n",
      "\\[\n",
      "\\Rightarrow \\frac{a}{(a-b)(a-c)} - \\frac{b}{(b-c)(a-c)} = \\frac{c}{(a-b)(b-c)} - \\frac{b}{(a-c)(b-c)} = 0\n",
      "\\]\n",
      "\n",
      "c) \\[\n",
      "\\frac{x^2}{x-1} - \\frac{x^3}{x^2-1} = \\frac{x^3 - x^2 + x}{(x-1)(x^2+x+1)} = \\frac{1}{x^2 - x}\n",
      "\\]\n",
      "\n",
      "d) \\[\n",
      "(a+b+c+d)^4 (a-b+c+d)^2 \\left( (a+b+c+d)^2 \\right) \\left( (a-b-c-d)^2 \\right)\n",
      "\\]\n",
      "\n",
      "\\[\n",
      "a^4 + b^4 + c^4 + d^4 + 4a^3b + 4a^3c + 4a^3d + 6a^2b^2 + 6a^2c^2 + 6a^2d^2 + 4ab^3 + 4ac^3 + 4ad^3 + b^4 + c^4 + d^4\n",
      "\\]\n",
      "\n",
      "\\[\n",
      "+ 4a^3b + 4a^3c + 4a^3d + 6a^2b^2 + 6a^2c^2 + 6a^2d^2 + 4ab^3 + 4ac^3 + 4ad^3 + b^4 + c^4 + d^4\n",
      "\\]\n",
      "\n",
      "\\[\n",
      "\\Rightarrow 4a^2 + 4b^2 + 4c^2 + 4d^2\n",
      "\\]\n",
      "\n",
      "\\[\n",
      "\\Rightarrow 4 \\left( a^2 + b^2 + c^2 + d^2 \\right)\n",
      "\\]\n",
      "\n",
      "\\end{document}\n",
      "```\n",
      "yay\n"
     ]
    }
   ],
   "source": [
    "# loop\n",
    "while n < len(doc):\n",
    "\tpix = doc[n].get_pixmap().pil_image()\n",
    "\tpix.save(f\"./images/from_pdfs/{direc}/page-{n+1}.png\")\n",
    "\tb64_image = img_to_b64(f\"./images/from_pdfs/{direc}/page-{n+1}.png\")\n",
    "\tprompt = read_file(\"./prompts/latex_gen.md\")\n",
    "\tresp, use = gpt.ask_LLM_txt_and_img(prompt, b64_image, temperature=0)\n",
    "\twith open(f\"./images/from_pdfs/{direc}/page-{n+1}.txt\", \"w\") as f:\n",
    "\t\tf.write(resp)\n",
    "\tn += 1"
   ]
  }
 ],
 "metadata": {
  "kernelspec": {
   "display_name": ".venv",
   "language": "python",
   "name": "python3"
  },
  "language_info": {
   "codemirror_mode": {
    "name": "ipython",
    "version": 3
   },
   "file_extension": ".py",
   "mimetype": "text/x-python",
   "name": "python",
   "nbconvert_exporter": "python",
   "pygments_lexer": "ipython3",
   "version": "3.10.8"
  }
 },
 "nbformat": 4,
 "nbformat_minor": 5
}
