\documentclass{article}
\usepackage{amsmath, amssymb}
\begin{document}

\section*{MÃ©thode de substitution (Analyse)}

Si $F(x)$ est une primitive de $f(x)$, on a :
\[
F(x) = \int f(x) \, dx \quad \Leftrightarrow \quad f(x) = \frac{d}{dx} F(x)
\]

Si on pose $x = g(t)$, alors :
\[
\frac{d}{dx} F(g(t)) = f(g(t)) \cdot g'(t) \Rightarrow \int f(g(t)) \cdot g'(t) \, dt = F(g(t)) + C
\]

\[
\boxed{\int f(x) \, dx = \int f(g(t)) \cdot g'(t) \, dt}
\]

\subsection*{Exemple}

\[
\int \frac{1}{\sqrt{x} + 1} \, dx
\Rightarrow t = \sqrt{x} \Rightarrow x = t^2 \Rightarrow dx = 2t \, dt
\]

\[
\int \frac{1}{t + 1} \cdot 2t \, dt = 2 \int \frac{t}{t + 1} \, dt
= 2 \int \left( 1 + \frac{t - 1}{t + 1} \right) dt
\]

\[
= 2 \left( t - \ln(t + 1) \right) + C
\]

\end{document}
