\documentclass{article}
\usepackage{amsmath}
\begin{document}

\noindent
MÃ©thode de substitution \hfill \textnormal{Analyse}

\medskip

\noindent
Si $F(x)$ est une primitive de $f(x)$, on a 
\[
F(x) = \int f(x) \, dx \iff f(x) = \frac{d}{dx}F(x)
\]

\noindent
si on pose $\boxed{x = g(t)}$, alors
\[
\frac{d}{dx} F(g(t)) = f(g(t)) \cdot g'(t) \iff \int f(g(t)) \cdot g'(t) \, dt = F(g(t)) + C
\]

\noindent
On a donc 
\[
\boxed{\int f(x) \, dx = \int f(g(t)) \cdot g'(t) \, dt}
\]

\bigskip

\noindent
Ex:
\[
\int \frac{1}{\sqrt{x + 1}} \, dx = \Rightarrow t = \sqrt{x}, \quad x = t^2, \quad dx = 2t \, dt
\]

\noindent
\[
\implies \int \frac{1}{\sqrt{x + 1}} \, dx = \int \frac{1}{t^2 + 1} \cdot 2t\, dt = 2 \int \frac{t}{t^2 + 1} dt
\]

\noindent
\[
= 2 \int \left( 1 + \frac{-1}{t^2 + 1} \right) dt = 2 \cdot \left( t - \ln(t^2 + 1) \right) + C
\]

\end{document}